HML as a specific unary logic

Cslib/Foundations/Data/PFunctor/Basic.lean
@@ -8,11 +8,17 @@ module
 
 public import Mathlib.Data.PFunctor.Univariate.Basic
 
-/-! # Additional basic definitions on polynomial functors -/
+/-! # Additional basic theory on polynomial functors -/
 
 @[expose] public section
 
 namespace PFunctor
+
+/-- The constant child map for `a`. -/
+def const {P : PFunctor} (a : P.A) (x : α) : P.B a → α := fun _ => x
+
+@[simp, scoped grind =]
+theorem const_apply {P : PFunctor} (a : P.A) (x : α) (i : P.B a) : PFunctor.const a x i = x := rfl
 
 section Unary
 
@@ -36,6 +42,16 @@ attribute [instance_reducible, instance] DecidableEqChildren.decidableEq
 /-- A unary polynomial functor has decidable child equality. -/
 instance (P : PFunctor) [P.Unary] : P.DecidableEqChildren where
   decidableEq _ _ _ := isTrue (Subsingleton.elim _ _)
+
+/-- Constructs a unary polynomial functor. -/
+abbrev mkUnary (A : Type*) : PFunctor where
+  A := A
+  B := fun _ => Unit
+
+instance {A : Type u} : (mkUnary A).Unary where
+  unary _ := by
+    change Unique Unit
+    infer_instance
 
 end Unary
 
