Cslib/Logics/HML/Basic.lean
@@ -7,8 +7,9 @@ Authors: Fabrizio Montesi, Marco Peressotti, Alexandre Rademaker
 module
 
 public import Cslib.Foundations.Semantics.LTS.Bisimulation
-public import Cslib.Foundations.Logic.Operators
-public import Cslib.Foundations.Logic.InferenceSystem
+public import Cslib.Foundations.Semantics.Frame.LTS
+public import Cslib.Logics.Modal.Semantics
+public import Cslib.Logics.Modal.Unary.LTS
 
 /-! # Hennessy-Milner Logic (HML)
 
@@ -47,252 +48,52 @@ distinguishing proposition that one state satisfies and the other does not.
 
 @[expose] public section
 
-namespace Cslib.Logic.HML
+namespace Cslib.Logic.Modal
+
+open PFunctor
+
+namespace HML
 
 /-- Propositions. -/
-inductive Proposition (Label : Type u) : Type u where
-  /-- Truth. -/
-  | true
-  /-- Conjunction. -/
-  | and (φ₁ φ₂ : Proposition Label)
-  /-- Negation. -/
-  | not (φ : Proposition Label)
-  /-- Possibility (dynamic diamond modality). -/
-  | diamond (μ : Label) (φ : Proposition Label)
-
-instance : Top (Proposition Label) := ⟨.true⟩
-instance : HasAnd (Proposition Label) := ⟨.and⟩
-instance : HasNot (Proposition Label) := ⟨.not⟩
-instance : HasDynamicDiamond (Proposition Label) Label := ⟨.diamond⟩
-
-/-- Falsity, derived from negation and truth. -/
-@[match_pattern]
-def Proposition.false : Proposition Label := ¬⊤
-
-instance : Bot (Proposition Label) := ⟨.false⟩
-
-/-- Disjunction, derived from negation and conjunction. -/
-@[match_pattern]
-def Proposition.or (φ₁ φ₂ : Proposition Label) : Proposition Label := ¬(¬φ₁ ∧ ¬φ₂)
-
-instance : HasOr (Proposition Label) := ⟨Proposition.or⟩
-
-/-- Implication. -/
-@[match_pattern]
-def Proposition.imp (φ₁ φ₂ : Proposition Label) : Proposition Label := ¬φ₁ ∨ φ₂
-
-instance : HasImp (Proposition Label) := ⟨.imp⟩
-
-/-- Bi-implication. -/
-@[match_pattern]
-def Proposition.iff (φ₁ φ₂ : Proposition Label) : Proposition Label := (φ₁ → φ₂) ∧ (φ₂ → φ₁)
-
-instance : HasIff (Proposition Label) := ⟨.iff⟩
-
-/-- Necessity (dynamic box modality), derived from dynamic diamond and negation. -/
-@[match_pattern]
-def Proposition.box (μ : Label) (φ : Proposition Label) : Proposition Label := ¬d⟨μ⟩¬φ
-
-instance : HasDynamicBox (Proposition Label) Label := ⟨.box⟩
-
-@[scoped grind =]
-lemma Proposition.top_def : .true = ((⊤ : Proposition Label)) := rfl
-
-@[scoped grind =]
-lemma Proposition.bot_def : .false = ((⊥ : Proposition Label)) := rfl
-
-@[scoped grind =]
-lemma Proposition.and_def (φ₁ φ₂ : Proposition Label) : φ₁.and φ₂ = (φ₁ ∧ φ₂) := rfl
-
-@[scoped grind =]
-lemma Proposition.not_def (φ : Proposition Label) : φ.not = ¬φ := rfl
-
-@[scoped grind =]
-lemma Proposition.diamond_def (μ : Label) (φ : Proposition Label) :
-  Proposition.diamond μ φ = d⟨μ⟩φ := rfl
-
-@[scoped grind =]
-lemma Proposition.or_def (φ₁ φ₂ : Proposition Label) : φ₁.or φ₂ = (φ₁ ∨ φ₂) := rfl
-
-@[scoped grind =]
-lemma Proposition.imp_def (φ₁ φ₂ : Proposition Label) : φ₁.imp φ₂ = (φ₁ → φ₂) := rfl
-
-@[scoped grind =]
-lemma Proposition.iff_def (φ₁ φ₂ : Proposition Label) :
-    φ₁.iff φ₂ = (φ₁ ↔ φ₂) := rfl
-
-@[scoped grind =]
-lemma Proposition.box_def (μ : Label) (φ : Proposition Label) : Proposition.box μ φ = d[μ]φ := rfl
+abbrev Proposition (Label Atom : Type*) := Modal.Proposition (mkUnary Label) Atom
 
 /-- Finite conjunction of propositions. -/
 @[simp, scoped grind =]
-def Proposition.finiteAnd (φs : List (Proposition Label)) : Proposition Label :=
+def Proposition.finiteAnd (φs : List (Proposition Label Atom)) : Proposition Label Atom :=
   List.foldr (· ∧ ·) ⊤ φs
 
 /-- Finite disjunction of propositions. -/
 @[simp, scoped grind =]
-def Proposition.finiteOr (φs : List (Proposition Label)) : Proposition Label :=
+def Proposition.finiteOr (φs : List (Proposition Label Atom)) : Proposition Label Atom :=
   List.foldr (· ∨ ·) ⊥ φs
 
-/-- Satisfaction relation. `Satisfies lts s φ` means that, in the LTS `lts`, the state `s` satisfies
-the proposition `φ`. -/
-@[scoped grind]
-def Satisfies (lts : LTS State Label) (s : State) : Proposition Label → Prop
-  | .true => True
-  | .and φ₁ φ₂ => Satisfies lts s φ₁ ∧ Satisfies lts s φ₂
-  | .not φ => ¬Satisfies lts s φ
-  | .diamond μ φ => ∃ s', lts.Tr s μ s' ∧ Satisfies lts s' φ
+end HML
 
-/-- Judgement, representing the conclusions one reaches in HML. -/
-structure Judgement State Label where
-  /-- Constructs a judgement. -/
-  mk ::
-  /-- LTS. -/
-  lts : LTS State Label
-  /-- The state satisfying the proposition `φ`. -/
-  state : State
-  /-- The proposition satisfied by the state `s`. -/
-  φ : Proposition Label
+open Model HML LTS
+open scoped HML.Proposition Modal.Proposition InferenceSystem Satisfies Frame LTS
 
-@[inherit_doc] scoped notation "HML[" lts "," s " ⊨ " φ "]" => Judgement.mk lts s φ
-
-/-- Satisfaction for judgements. This just refers to the unbundled `Satisfies`. -/
-@[simp, scoped grind =]
-def Satisfies.Bundled (j : Judgement State Label) : Prop := Satisfies j.lts j.state j.φ
-
-instance : HasInferenceSystem (Judgement State Label) := ⟨Satisfies.Bundled⟩
-
-open scoped InferenceSystem Proposition
-
-@[scoped grind =]
-theorem derivation_def : Satisfies lts s φ = ⇓HML[lts,s ⊨ φ] := rfl
-
-@[scoped grind =]
-theorem Satisfies.not_iff_not : ⇓HML[lts,s ⊨ ¬φ] ↔ ¬⇓HML[lts,s ⊨ φ] := by rfl
-
-@[scoped grind .]
-theorem Satisfies.top : ⇓HML[lts,s ⊨ ⊤] := by
-  dsimp [Top.top]
-  grind [=_ derivation_def]
-
-@[scoped grind .]
-theorem Satisfies.bot : ¬⇓HML[lts,s ⊨ ⊥] := by
-  simp only [Bot.bot]
-  grind [= Proposition.false]
-
-@[scoped grind =]
-theorem Satisfies.and_iff_and :
-    ⇓HML[lts,s ⊨ φ₁ ∧ φ₂] ↔ ⇓HML[lts,s ⊨ φ₁] ∧ ⇓HML[lts,s ⊨ φ₂] := by rfl
-
-@[scoped grind =]
-theorem Satisfies.or_iff_or :
-    ⇓HML[lts,s ⊨ φ₁ ∨ φ₂] ↔ ⇓HML[lts,s ⊨ φ₁] ∨ ⇓HML[lts,s ⊨ φ₂] := by
-  grind [=_ Proposition.or_def, Proposition.or]
-
-@[scoped grind =]
-theorem Satisfies.diamond_iff_exists :
-    ⇓HML[lts,s ⊨ d⟨μ⟩φ] ↔ ∃ s', lts.Tr s μ s' ∧ ⇓HML[lts,s' ⊨ φ] := by rfl
-
-/-- Characterisation of the `→` connective.
-
-Implication is defined in terms of the more primitive connectives given in `Proposition`.
-This result proves that the definition is correct.
--/
-@[scoped grind =]
-theorem Satisfies.imp_iff_imp :
-    ⇓HML[lts,s ⊨ φ₁ → φ₂] ↔ (⇓HML[lts,s ⊨ φ₁] → ⇓HML[lts,s ⊨ φ₂]) := by
-  grind [=_ Proposition.imp_def, Proposition.imp]
-
-/-- Characterisation of the `↔` connective.
-
-Bi-implication is defined in terms of the more primitive connectives given in `Proposition`.
-This result proves that the definition is correct. -/
-@[scoped grind =]
-theorem Satisfies.iff_iff_iff :
-    ⇓HML[lts,s ⊨ φ₁ ↔ φ₂] ↔ (⇓HML[lts,s ⊨ φ₁] ↔ ⇓HML[lts,s ⊨ φ₂]) := by
-  simp only [HasIff.iff, Proposition.iff]
-  grind
-
-@[scoped grind =]
-theorem Satisfies.box_iff_forall :
-    ⇓HML[lts,s ⊨ d[μ]φ] ↔ ∀ s', lts.Tr s μ s' → ⇓HML[lts,s' ⊨ φ] := by
-  grind [=_ Proposition.box_def, Proposition.box]
+variable {lts : LTS State Label} {v : State → Atom → Prop}
 
 /-- A state satisfies a finite conjunction iff it satisfies all conjuncts. -/
 @[scoped grind =]
 theorem Satisfies.finiteAnd_iff_forall :
-    ⇓HML[lts,s ⊨ Proposition.finiteAnd φs] ↔ ∀ φ ∈ φs, ⇓HML[lts,s ⊨ φ] := by
+    ⇓Modal[ofLTS lts v,s ⊨ Proposition.finiteAnd φs] ↔ ∀ φ ∈ φs, ⇓Modal[ofLTS lts v,s ⊨ φ] := by
   induction φs <;> grind
 
 /-- A state satisfies a finite disjunction iff it satisfies some disjunct. -/
 @[scoped grind =]
 theorem Satisfies.finiteOr_iff_exists :
-    ⇓HML[lts,s ⊨ Proposition.finiteOr φs] ↔ ∃ φ ∈ φs, ⇓HML[lts,s ⊨ φ] := by
+    ⇓Modal[ofLTS lts v,s ⊨ Proposition.finiteOr φs] ↔ ∃ φ ∈ φs, ⇓Modal[ofLTS lts v,s ⊨ φ] := by
   induction φs <;> grind
-
-/-- Denotation of a proposition. -/
-@[simp, scoped grind =]
-def Proposition.denotation (lts : LTS State Label)
-    : Proposition Label → Set State
-  | .true => Set.univ
-  | .and φ₁ φ₂ => φ₁.denotation lts ∩ φ₂.denotation lts
-  | .not φ => (φ.denotation lts)ᶜ
-  | .diamond μ φ => {s | ∃ s', lts.Tr s μ s' ∧ s' ∈ φ.denotation lts}
-
-/-- The theory of a state is the set of all propositions that it satisfies. -/
-abbrev theory (lts : LTS State Label) (s : State) : Set (Proposition Label) :=
-  {φ | ⇓HML[lts,s ⊨ φ]}
-
-/-- Two states are theory-equivalent (for a specific LTS) if they have the same theory. -/
-abbrev TheoryEq (lts : LTS State Label) (s1 s2 : State) :=
-  theory lts s1 = theory lts s2
-
-open Proposition LTS
-
-/-- Characterisation theorem for the denotational semantics. -/
-@[scoped grind =]
-theorem mem_denotation_iff_satisfies {φ : Proposition Label} :
-    s ∈ φ.denotation lts ↔ ⇓HML[lts,s ⊨ φ] := by
-  induction φ generalizing s <;> grind [=_ derivation_def]
-
-@[scoped grind .]
-theorem mem_theory_iff_satisfies : φ ∈ theory lts s ↔ ⇓HML[lts,s ⊨ φ] := by
-  grind
-
-open scoped Satisfies
-
-/-- A state is in the denotation of a proposition iff it is not in the denotation of the negation
-of the proposition. -/
-@[scoped grind =]
-theorem not_denotation {lts : LTS State Label} (φ : Proposition Label) :
-    s ∉ (¬φ).denotation lts ↔ s ∈ φ.denotation lts := by grind
-
-/-- Two states are theory-equivalent iff they are denotationally equivalent. -/
-theorem theoryEq_denotation_eq {lts : LTS State Label} :
-    TheoryEq lts s1 s2 ↔
-    (∀ φ : Proposition Label, s1 ∈ φ.denotation lts ↔ s2 ∈ φ.denotation lts) := by
-  grind [=_ mem_theory_iff_satisfies, =_ mem_denotation_iff_satisfies]
-
-/-- If two states are not theory equivalent, there exists a distinguishing proposition. -/
-lemma not_theoryEq_satisfies (h : ¬TheoryEq lts s1 s2) :
-    ∃ φ, (⇓HML[lts,s1 ⊨ φ] ∧ ¬⇓HML[lts,s2 ⊨ φ]) := by
-  grind [=_ Satisfies.not_iff_not]
-
-/-- If two states are theory equivalent and the former satisfies a proposition, the latter does as
-well. -/
-theorem theoryEq_satisfies (h : TheoryEq lts s1 s2)
-    (hs : ⇓HML[lts,s1 ⊨ φ]) : ⇓HML[lts,s2 ⊨ φ] := by
-  unfold TheoryEq theory at h
-  rw [Set.ext_iff] at h
-  exact (h φ).mp hs
 
 section ImageToPropositions
 
-variable {lts : LTS State Label} (stateMap : lts.image s μ → Proposition Label)
-variable [finImage : Fintype (lts.image s μ)]
+variable {s : State} {μ : Label} {lts : LTS State Label}
+  (stateMap : lts.image s μ → HML.Proposition Label Atom)
+  [finImage : Fintype (lts.image s μ)]
 
 /-- The list of propositions over finite μ-derivatives. -/
-noncomputable def propositions : List (Proposition Label) :=
+noncomputable def propositions : List (HML.Proposition Label Atom) :=
   finImage.elems.toList.map stateMap
 
 theorem propositions_complete (s' : lts.image s μ) : stateMap s' ∈ propositions stateMap := by
@@ -300,9 +101,9 @@ theorem propositions_complete (s' : lts.image s μ) : stateMap s' ∈ propositio
   use s', Finset.mem_toList.mpr (Fintype.complete s')
 
 theorem propositions_satisfies_conjunction (htr : lts.Tr s1 μ s1')
-    (hdist_spec : ∀ s2', ⇓HML[lts,s1' ⊨ (stateMap s2')]) :
-    ⇓HML[lts,s1 ⊨ d⟨μ⟩finiteAnd (propositions stateMap)] := by
-  rw [Satisfies.diamond_iff_exists]
+    (hdist_spec : ∀ s2', ⇓Modal[ofLTS lts v,s1' ⊨ (stateMap s2')]) :
+    ⇓Modal[ofLTS lts v,s1 ⊨ d⟨μ⟩(Proposition.finiteAnd (propositions stateMap))] := by
+  rw [Satisfies.dynDiamond_iff_exists]
   use s1', htr
   rw [Satisfies.finiteAnd_iff_forall]
   intro φ hφ_mem
@@ -311,59 +112,67 @@ theorem propositions_satisfies_conjunction (htr : lts.Tr s1 μ s1')
 end ImageToPropositions
 
 /-- Theory equivalence is a bisimulation. -/
-@[scoped grind ⇒]
-theorem theoryEq_isBisimulation (lts : LTS State Label)
+theorem theoryEq_isBisimulation
     [image_finite : ∀ s μ, Finite (lts.image s μ)] :
-    lts.IsHomBisimulation (TheoryEq lts) := by
+    lts.IsHomBisimulation (TheoryEq (ofLTS lts v)) := by
   intro s1 s2 h μ
   let (s : State) := @Fintype.ofFinite (lts.image s μ) (image_finite s μ)
   constructor
   case left =>
     intro s1' htr
     by_contra
-    have hdist : ∀ s2' : lts.image s2 μ, ∃ φ, ⇓HML[lts,s1' ⊨ φ] ∧ ¬⇓HML[lts,s2'.val ⊨ φ] := by
+    have hdist : ∀ s2' : lts.image s2 μ, ∃ φ, ⇓Modal[ofLTS lts v,s1' ⊨ φ] ∧
+        ¬⇓Modal[ofLTS lts v,s2'.val ⊨ φ] := by
       intro ⟨s2', hs2'⟩
       apply not_theoryEq_satisfies
       grind
     choose dist_formula hdist_spec using hdist
     let conjunction := Proposition.finiteAnd (propositions dist_formula)
-    have hs1_diamond : ⇓HML[lts,s1 ⊨ d⟨μ⟩conjunction] := by
+    have hs1_diamond : ⇓Modal[ofLTS lts v,s1 ⊨ d⟨μ⟩conjunction] := by
       grind [propositions_satisfies_conjunction]
-    obtain ⟨s2'', htr2, hsat⟩ := Satisfies.diamond_iff_exists.mp (theoryEq_satisfies h hs1_diamond)
+    obtain ⟨s2'', htr2, hsat⟩ := Satisfies.dynDiamond_iff_exists.mp
+      (theoryEq_satisfies h hs1_diamond)
     grind [propositions_complete dist_formula ⟨s2'', htr2⟩]
   case right =>
     -- Symmetric to left case
     intro s2' htr
     by_contra
-    have hdist : ∀ s1' : lts.image s1 μ, ∃ a, Satisfies lts s2' a ∧ ¬Satisfies lts s1'.val a := by
+    have hdist : ∀ s1' : lts.image s1 μ, ∃ a, ⇓Modal[ofLTS lts v, s2' ⊨ a] ∧
+        ¬⇓Modal[ofLTS lts v, s1'.val ⊨ a] := by
       intro ⟨s1', hs1'⟩
       apply not_theoryEq_satisfies
       grind
     choose dist_formula hdist_spec using hdist
     let conjunction := Proposition.finiteAnd (propositions dist_formula)
-    have hs2_diamond : ⇓HML[lts,s2 ⊨ d⟨μ⟩conjunction] := by
+    have hs2_diamond : ⇓Modal[ofLTS lts v,s2 ⊨ d⟨μ⟩conjunction] := by
       grind [propositions_satisfies_conjunction]
     obtain ⟨s1'', htr1, hsat⟩ :=
-      Satisfies.diamond_iff_exists.mp (theoryEq_satisfies h.symm hs2_diamond)
+      Satisfies.dynDiamond_iff_exists.mp (theoryEq_satisfies h.symm hs2_diamond)
     grind [propositions_complete dist_formula ⟨s1'', htr1⟩]
 
 /-- If two states are in a bisimulation, one satisfies a proposition iff the other does. -/
-@[scoped grind ⇒]
 lemma bisimulation_satisfies {hrb : lts.IsHomBisimulation r}
-    (hr : r s1 s2) (φ : Proposition Label) : ⇓HML[lts,s1 ⊨ φ] ↔ ⇓HML[lts,s2 ⊨ φ] := by
-  induction φ generalizing s1 s2 <;> grind [IsBisimulation]
+    (hv : ∀ {s1 s2}, r s1 s2 → ∀ p, v s1 p ↔ v s2 p) (hr : r s1 s2)
+    (φ : HML.Proposition Label Atom) :
+    ⇓Modal[ofLTS lts v,s1 ⊨ φ] ↔ ⇓Modal[ofLTS lts v,s2 ⊨ φ] := by
+  induction φ generalizing s1 s2 with
+  | triangle =>
+    rw [Proposition.triangle_def, Proposition.unary_triangle_eq_dynDiamond]
+    grind only [IsBisimulation, Satisfies.ofLTS_dynDiamond_iff_exists]
+  | _ => grind
 
-lemma bisimulation_theoryEq {hrb : lts.IsHomBisimulation r} (hr : r s1 s2) :
-    TheoryEq lts s1 s2 := by grind
+lemma bisimulation_theoryEq {hrb : lts.IsHomBisimulation r}
+    (hv : ∀ {s1 s2}, r s1 s2 → ∀ p, v s1 p ↔ v s2 p) (hr : r s1 s2) :
+    TheoryEq (ofLTS lts v) s1 s2 := by grind [bisimulation_satisfies]
 
 /-- Theory equivalence and bisimilarity coincide for image-finite LTSs. -/
-theorem theoryEq_eq_bisimilarity {lts : LTS State Label}
-    [image_finite : ∀ s μ, Finite (lts.image s μ)] :
-    TheoryEq lts = HomBisimilarity lts := by
+theorem theoryEq_eq_bisimilarity
+    [image_finite : ∀ s μ, Finite (lts.image s μ)]
+    (hv : ∀ {s1 s2}, s1 ~[lts] s2 → ∀ p, v s1 p ↔ v s2 p := by grind) :
+    TheoryEq (ofLTS lts v) = HomBisimilarity lts := by
   ext s1 s2
   apply Iff.intro <;> intro h
-  · exists TheoryEq lts
-    grind
-  · grind
+  · exact ⟨TheoryEq (ofLTS lts v), h, theoryEq_isBisimulation⟩
+  · grind [bisimulation_satisfies]
 
-end Cslib.Logic.HML
+end Cslib.Logic.Modal
