Cslib/Logics/Modal/Unary/Basic.lean
@@ -9,6 +9,7 @@ module
 public import Cslib.Foundations.Data.PFunctor.Basic
 public import Cslib.Logics.Modal.Basic
 public import Cslib.Logics.Modal.Semantics
+public import Cslib.Logics.Modal.LogicalEquivalence
 
 /-! # Unary Modal Logic -/
 
@@ -19,15 +20,34 @@ namespace Cslib.Logic.Modal
 open PFunctor
 open scoped InferenceSystem Proposition Satisfies Frame
 
-@[scoped grind =]
-theorem Satisfies.dynDiamond_iff_exists [Unary τ] {m : Model World τ Atom}
-    {φ : Proposition τ Atom} : ⇓Modal[m,w ⊨ d⟨op⟩φ] ↔
-      ∃ w', m.toFrame.diagonal op w w' ∧ ⇓Modal[m,w' ⊨ φ] := by
-  grind [Satisfies.triangle_iff_exists]
+variable {τ : PFunctor} [τ.Unary]
+
+/-- Context constructor for the dynamic diamond modality. -/
+@[match_pattern]
+def Proposition.Context.dynDiamond (c : Context τ Atom) (a : τ.A) : Context τ Atom :=
+  .triangle a default c fun ⟨i, hi⟩ => (hi (Subsingleton.elim i default)).elim
 
 @[scoped grind =]
-theorem Satisfies.dynBox_iff_forall [Unary τ] {m : Model World τ Atom} {φ : Proposition τ Atom} :
-    ⇓Modal[m,w ⊨ d[op]φ] ↔ ∀ w', m.toFrame.diagonal op w w' → ⇓Modal[m,w' ⊨ φ] := by
-  grind [Frame.diagonal]
+theorem Proposition.unary_triangle_eq_dynDiamond {a : τ.A}
+    (φs : PropositionMap τ a Atom) : (Δ[a]φs) = d⟨a⟩(φs default) := by
+  rw [PFunctor.Unary.fun_eq_const a φs]
+  rfl
+
+@[modal =]
+theorem Satisfies.dynDiamond_iff_exists {m : Model World τ Atom}
+    {φ : Proposition τ Atom} : ⇓Modal[m,w ⊨ d⟨a⟩φ] ↔
+      ∃ w', m.toFrame.diagonal a w w' ∧ ⇓Modal[m,w' ⊨ φ] := by grind
+
+@[modal =]
+theorem Satisfies.dynBox_iff_forall {m : Model World τ Atom} {φ : Proposition τ Atom} :
+    ⇓Modal[m,w ⊨ d[a]φ] ↔ ∀ w', m.toFrame.diagonal a w w' → ⇓Modal[m,w' ⊨ φ] := by grind
+
+omit [τ.Unary] in
+/-- The dual axiom (reformulated for unary modal logic). -/
+theorem Satisfies.unary_dual (f : Frame World τ) {a : τ.A} {φ : Proposition τ Atom} :
+    Axiom f⇓(d⟨a⟩φ ↔ ¬d[a]¬φ) := by
+  /- We use `grind only` on purpose here because this axiom should be derivable from the more
+    more general `Satisfies.dual`. -/
+  grind only [modal, Satisfies.dual]
 
 end Cslib.Logic.Modal
