CslibTests/HML.lean
@@ -5,16 +5,24 @@ Authors: Fabrizio Montesi
 -/
 
 import Cslib.Logics.HML.Basic
-import Cslib.Logics.HML.LogicalEquivalence
+import Cslib.Logics.Modal.LogicalEquivalence
 import Cslib.Languages.CCS.Semantics
 
 namespace CslibTests
 
-open Cslib Logic HML LTS
+open Cslib Logic Modal HML LTS Model Proposition Satisfies
+open scoped InferenceSystem
 
 example [∀ p μ, Finite ((CCS.lts (defs := defs)).image p μ)] :
-    TheoryEq (CCS.lts (defs := defs)) = HomBisimilarity (CCS.lts (defs := defs)) :=
+    TheoryEq (Atom := Unit) (ofLTS (CCS.lts (defs := defs)) (fun _ _ => True)) =
+      HomBisimilarity (CCS.lts (defs := defs)) :=
   theoryEq_eq_bisimilarity ..
+
+example (v : State → Atom → Prop) (htr : lts.Tr s μ s') (hφ : ⇓Modal[ofLTS lts v,s' ⊨ φ]) :
+    ⇓Modal[ofLTS lts v,s ⊨ d⟨μ⟩φ] := by grind only [modal]
+
+example (v : State → Atom → Prop) (hbox : ⇓Modal[Model.ofLTS lts v,s ⊨ d[μ]φ])
+    (htr : lts.Tr s μ s') : ⇓Modal[ofLTS lts v,s' ⊨ φ] := by grind only [modal]
 
 section LogicalEquivalence
 
@@ -26,21 +34,23 @@ with grind. Note that the grind proof works because Satisfies.and_iff_and gives 
 principle on the satisfaction relation for the and-connective.
 -/
 
-open scoped InferenceSystem
-open Proposition
+open PFunctor
 
-example {State : Type u} {lts : LTS State Label} {s : State} {μ : Label} {φ₁ φ₂ : Proposition Label}
-    (h : ⇓HML[lts,s ⊨ (d⟨μ⟩φ₁) ∧ φ₂])
-    : ⇓HML[lts,s ⊨ (¬d[μ]¬φ₁) ∧ φ₂] := by
-  let pc : HasContext.Context (Proposition Label) := Context.andL .hole φ₂
+example {State : Type u} {lts : LTS State Label} {s : State} {μ : Label}
+    {φ₁ φ₂ : HML.Proposition Label Atom} (v : State → Atom → Prop)
+    (h : ⇓Modal[ofLTS lts v,s ⊨ (d⟨μ⟩φ₁) ∧ φ₂]) : ⇓Modal[ofLTS lts v,s ⊨ (¬d[μ]¬φ₁) ∧ φ₂] := by
+  let pc : HasContext.Context (HML.Proposition Label Atom) := Context.andL .hole φ₂
+  have dual a (φ : HML.Proposition Label Atom) : d⟨a⟩φ ≡[UEquiv (World := State)] ¬d[a]¬φ := by
+    grind only [modal, Satisfies.unary_dual]
   have eqv := LawfulCongruence.covariant.elim pc (dual μ φ₁)
-  let jc : HasHContext.Context (Judgement State Label) (Proposition Label) :=
-    Judgement.Context.mk lts s
+  let jc : HasHContext.Context (Judgement State (mkUnary Label) Atom)
+      (HML.Proposition Label Atom) := Judgement.Context.mk (ofLTS lts v) s
   apply LogicalEquivalence.eqvFillValid eqv jc h
 
-example {State : Type u} {lts : LTS State Label} {s : State} {μ : Label} {φ₁ φ₂ : Proposition Label}
-    (h : ⇓HML[lts,s ⊨ (d⟨μ⟩φ₁) ∧ φ₂]) : ⇓HML[lts,s ⊨ (¬d[μ]¬φ₁) ∧ φ₂] := by
-  grind only [= Satisfies.and_iff_and, => equiv_iff, dual μ φ₁ lts]
+example {State : Type u} {lts : LTS State Label} {s : State} {μ : Label}
+    {φ₁ φ₂ : HML.Proposition Label Atom} (v : State → Atom → Prop)
+    (h : ⇓Modal[ofLTS lts v,s ⊨ (d⟨μ⟩φ₁) ∧ φ₂]) :
+    ⇓Modal[ofLTS lts v,s ⊨ (¬d[μ]¬φ₁) ∧ φ₂] := by grind [modal]
 
 end LogicalEquivalence
 
